theories/sim/one_step.v
@@ -27,6 +27,27 @@ Proof.
   apply (UPD O (Some r_f)); [by apply cmra_discrete_valid_iff|by rewrite /= comm].
 Qed.
 
+Lemma sim_body_post_mono fs ft r n es σs et σt Φ Φ' :
+  Φ' <6= Φ →
+  r ⊨{n,fs,ft} (es, σs) ≥ (et, σt) : Φ' →
+  r ⊨{n,fs,ft} (es, σs) ≥ (et, σt) : Φ.
+Proof.
+  revert r n es σs et σt Φ Φ'. pcofix CIH. intros r0 n es σs et σt Φ Φ' LE SIM.
+  pfold. punfold SIM.
+  intros NT r_f WSAT. specialize (SIM NT r_f WSAT) as [NOTS TE SIM].
+  constructor; [done|..].
+  { intros.
+    destruct (TE _ TERM) as (vs' & σs' & r' & idx' & STEP' & WSAT' & HΦ').
+    naive_solver. }
+  inversion SIM.
+  - left. intros.
+    specialize (STEP _ _ STEPT) as (es' & σs' & r' & idx' & STEP' & WSAT' & SIM').
+    exists es', σs', r', idx'. do 2 (split; [done|]).
+    pclearbot. right. eapply CIH; eauto.
+  - econstructor 2; eauto. intros.
+    destruct (CONT _ _ _ σs' σt' VRET) as [idx' SIM'].
+    exists idx'. pclearbot. right. eapply CIH; eauto.
+Qed.
 
 Lemma sim_body_bind fs ft r n
   (Ks: list (ectxi_language.ectx_item (bor_ectxi_lang fs)))
