theories/sim/program.v
@@ -1,0 +1,31 @@
+From stbor.lang Require Import steps_wf steps_inversion.
+From stbor.sim Require Import sflib behavior global local invariant global_adequacy local_adequacy one_step.
+
+Set Default Proof Using "Type".
+
+Lemma sim_prog_sim
+      prog_src `{NSD: ∀ e σ, Decision (never_stuck prog_src e σ)}
+      prog_tgt
+      (FUNS: sim_local_funs wsat vrel_expr prog_src prog_tgt end_call_sat)
+      (MAINT: ∃ ebt HCt, prog_tgt !! "main" = Some (@FunV [] ebt HCt))
+  : behave_prog prog_tgt <1= behave_prog prog_src.
+Proof.
+  destruct MAINT as (ebt & HCt & Eqt).
+  destruct (FUNS _ _ Eqt) as ([xls ebs HCs] & Eqs & Eql & SIMf).
+  apply nil_length_inv in Eql. subst xls.
+  specialize (SIMf ε ebs ebt [] [] init_state init_state) as [idx SIM]; [done..|].
+  unfold behave_prog. eapply (adequacy _ _ idx); [apply _| |by apply wf_init_state..].
+  eapply sim_local_conf_sim; eauto.
+  econs; eauto; swap 2 4.
+  - econs 1.
+  - ss.
+  - ss.
+  - eapply (sim_body_step_into_call _ _ _ _ _ [] ebs HCs [] ebs [] ebt HCt [] ebt);
+      [done..|].
+    eapply (sim_body_bind _ _ _ _ [EndCallCtx] [EndCallCtx] (InitCall ebs) (InitCall ebt)).
+    eapply sim_body_post_mono; [|exact SIM].
+    clear SIM. simpl.
+    intros r1 idx1 vs σs vt σt [ESAT (v1 & v2 & Eq1 & Eq2 & VREL)].
+    rewrite Eq1 Eq2. by apply sim_body_end_call.
+  - rewrite right_id. apply wsat_init_state.
+Qed.
